CompatibilityDefinition

src/Spec/update.v
@@ -3,7 +3,7 @@ Require Import Spec.Proc.
 Require Import Spec.ProcTheorems.
 Require Import Helpers.RelationAlgebra.
 Require Import Helpers.RelationRewriting.
-Import  RelationNotations. 
+Import  RelationNotations.
 
 Section Updates.
 
@@ -15,15 +15,15 @@ Variable  Op1: Type -> Type.
 
 Variable  O': Type -> Type.
 
-Inductive  Op2: Type -> Type :=
-| Op1case(T:Type) : Op1 T -> Op2 T
-| O'case(T:Type) : O' T -> Op2 T. 
+Inductive  COP: Type -> Type :=
+| Op1case(T:Type) : Op1 T -> COP T
+| O'case(T:Type) : O' T -> COP T. 
 
 Variable  Lc : Layer Op.
 
 Variable LA1: Layer Op1.
 
-Variable LA2: Layer Op2.
+Variable LA2: Layer COP.
 
 Print relation. 
 
@@ -31,7 +31,7 @@ Variable shutdown: relation Lc.(State) Lc.(State) unit.
 
 Print proc. 
 
-Fixpoint  relinkingFunction {T: Type} (p: proc Op1 T) : proc Op2 T :=
+Fixpoint  relinkingFunction {T: Type} (p: proc Op1 T) : proc COP T :=
   match p with
   | Call o => Call (Op1case o)
   | Ret v => Ret v
@@ -44,9 +44,124 @@ Search "compile".
 
 About compile.
 
-About exec. 
+Definition compatibleUpdate  (M1 : LayerImpl Op Op1) (M2 : LayerImpl Op Op1) (R1: relation LA1.(State) Lc.(State) unit) (R2: relation LA1.(State) Lc.(State) unit) :=
+  forall (T:Type) (p: proc Op1 T), forall (s1 s2 c1: Lc.(State)) (state : LA1.(State)) (r:T),
+  ((exec Lc.(sem) (compile M2 p)) (s1) (s2) (r) /\ R2 (state) (s1) (tt)  /\ R1 (state) (c1) (tt) ) ->
+  exists (state' : LA1.(State)) (c2: Lc.(State)), (exec Lc.(sem) (compile M1 p)) (c1) (c2) (r) /\ (exec LA1.(sem) p ) (state) (state') (r) /\ R2 (state') (s2) (tt) /\ R1 (state') (c2) (tt). 
 
-Definition softwareUpdate(M1: LayerImpl Op  Op1) (M2: LayerImpl Op  Op2):=
+Theorem updateOP : forall (T:Type) (op: Op1 T) (M1 : LayerImpl Op Op1) (M2 : LayerImpl Op Op1) (R1: relation LA1.(State) Lc.(State) unit) (R2: relation LA1.(State) Lc.(State) unit) (s1 s2 c1: Lc.(State)) (state : LA1.(State)) (r:T),
+  exec Lc (compile M2 (Call op)) s1 s2 r /\ R2 state s1 tt /\ R1 state c1 tt ->
+  exists (state' : LA1.(State)) (c2 : Lc.(State)),
+    exec Lc (compile M1 (Call op)) c1 c2 r /\
+    exec LA1 (Call op) state state' r /\ R2 state' s2 tt /\ R1 state' c2 tt.
+Proof.
+  Admitted. 
+
+Theorem compatibleUpdateProof1: forall (M1 : LayerImpl Op Op1) (M2 : LayerImpl Op Op1) (R1: relation LA1.(State) Lc.(State) unit) (R2: relation LA1.(State) Lc.(State) unit), compatibleUpdate M1 M2 R1 R2.
+Proof.
+  intros. unfold compatibleUpdate. induction p.
+  - apply updateOP. 
+  - intros. destruct H as [H1 [H2 H3]]. simpl in H1. unfold pure in H1. destruct H1 as [H0 H1].
+    exists state. exists c1. split.
+    + simpl. unfold pure. auto. 
+    + split.
+      ++ simpl. unfold pure. auto. 
+      ++ split.
+         +++ rewrite -> H0 in H2.  assumption.
+         +++ assumption. 
+  - intros. destruct H0 as [H1 [H2 H3]].  simpl in H1. unfold and_then in H1.
+    destruct H1 as [o1 H1]. destruct H1 as [y [H1 H4]]. specialize IHp with s1 y c1 state o1.
+  assert (exec Lc (compile M2 p) s1 y o1 /\ R2 state s1 tt /\ R1 state c1 tt) as IH by (repeat (split; try assumption)). 
+    (* remember (IHp (conj (H1) (conj H2 H3))) as XXX . *)
+    apply IHp in IH. destruct IH as [state' IH]. destruct IH as [c2 IH].
+    specialize H with o1 y s2 c2 state' r. destruct IH as [IH [H5 H6]].
+    assert ( exec Lc (compile M2 (p2 o1)) y s2 r /\ R2 state' y tt /\ R1 state' c2 tt) as IH' by (repeat (split; try assumption)). apply H in IH'. destruct IH' as [state'' IH']. destruct IH' as [c3 IH'].
+
+    exists state''. exists c3. destruct IH' as [IH' [H7 H8]].  split.
+    + simpl. unfold and_then. exists o1.  exists c2. split.
+      ++ assumption. 
+      ++ assumption. 
+    + split.
+      ++ simpl. unfold and_then. exists o1. exists state'. auto.  
+      ++ auto.
+Qed. 
+
+Print Layer.
+
+Definition CompatibleUpdateWithoutAbsr  (M1 : LayerImpl Op Op1) (M2 : LayerImpl Op Op1) :=
+  forall (T:Type) (p1 p2: proc Op1 T), forall (s s' s'' c'': Lc.(State)) (r r1 r2: T),
+  Lc.(initP) (s) /\ (exec Lc.(sem) (compile M1 p1)) (s) (s') (r) /\
+  shutdown (s') (s') (tt) /\  (exec Lc.(sem) (compile M1 p2)) (s') (s'') (r1) /\
+  (exec Lc.(sem) (compile M2 p2)) (s') (c'') (r2) ->
+  r1 = r2 . 
+
+Theorem CompatibleUpdateWithoutAbsrInductive : forall (M1 : LayerImpl Op Op1) (M2 : LayerImpl Op Op1),
+  CompatibleUpdateWithoutAbsr M1 M2.
+Proof.
+  intros. unfold CompatibleUpdateWithoutAbsr. intros.
+  Admitted. 
+  
+
+Definition HoareTriple {T: Type} (P Q: Lc.(State) ->  Prop) (M1 : LayerImpl Op Op1) (z: proc Op1 T) :=
+  forall (s s': Lc.(State)) (r: T), P (s) /\ (exec Lc.(sem) (compile M1 z)) (s) (s') (r) -> Q (s').
+
+Definition HoareTripleP {T: Type} (P Q: LA1.(State) ->  Prop) (z: proc Op1 T) :=
+  forall (s s': LA1.(State)) (r: T), P (s) /\ (exec LA1.(sem) z) (s) (s') (r) -> Q (s').
+
+Print LayerRefinement. 
+
+Theorem proofPreservation: forall (T:Type) (M1 : LayerImpl Op Op1) (M2 : LayerImpl Op Op1) (R1: relation LA1.(State) Lc.(State) unit) (R2: relation LA1.(State) Lc.(State) unit) (P Q: Lc.(State) ->  Prop)  (P' Q': LA1.(State) ->  Prop) (z: proc Op1 T),
+  HoareTriple P Q M1 z /\ compatibleUpdate M1 M2 R1 R2 -> HoareTriple P Q M2 z.
+Proof.
+  intros. destruct H as [H1 H2 ]. unfold HoareTriple. intros. 
+  unfold HoareTriple in H1. specialize H1 with s s' r.
+  unfold compatibleUpdate in H2.
+  specialize H2 with T z s s' s LA1.(State) r.
+  Admitted. 
+
+
+(** ------------------------------------ OLD----------------------------------------- *)
+
+Definition compatibleUpdate1  (M1 : LayerImpl Op Op1) (M2 : LayerImpl Op Op1) (R1: relation LA1.(State) Lc.(State) unit) (R2: relation LA1.(State) Lc.(State) unit) :=
+  forall (T:Type) (p: proc Op1 T) (s1 s2: Lc.(State)) (state : LA1.(State)) (r:T),  exists (c1 c2: Lc.(State)),
+  ((exec Lc.(sem) (compile M2 p)) (s1) (s2) (r) /\ R2 (state) (s1) (tt) ->  (exec Lc.(sem) (compile M1 p)) (c1) (c2) (r) /\ R1 (state) (c1) (tt) ) ->
+  exists state':LA1.(State), (exec LA1.(sem) p ) (state) (state') (r) /\ R2 (state') (s2) (tt) /\ R1 (state') (c2) (tt).
+
+Lemma updateOP1: forall (T:Type) (op: Op1 T) (M1 : LayerImpl Op Op1) (M2 : LayerImpl Op Op1) (R1: relation LA1.(State) Lc.(State) unit) (R2: relation LA1.(State) Lc.(State) unit) (s1 s2: Lc.(State)) (state : LA1.(State)) (r:T),
+  exists (c1 c2: Lc.(State)), (exec Lc (M2.(compile_op) op) s1 s2 r /\ R2 state s1 tt ->
+     exec Lc (M1.(compile_op) op) c1 c2 r /\ R1 state c1 tt) ->
+    exists state' : LA1.(State),
+      LA1.(step) op state state' r /\ R2 state' s2 tt /\ R1 state' c2 tt.
+Proof.
+  Admitted.
+
+Theorem compatibleUpdateProof1: forall (M1 : LayerImpl Op Op1) (M2 : LayerImpl Op Op1) (R1: relation LA1.(State) Lc.(State) unit) (R2: relation LA1.(State) Lc.(State) unit), compatibleUpdate1 M1 M2 R1 R2.
+Proof.
+  intros. unfold compatibleUpdate1. induction p as [ | | ]. 
+  - admit. 
+  - admit. (**simpl. unfold pure. exists s1.  exists s2. intros. exists state. assert ( (s1 = s2 /\ r = v) /\ R2 state s1 tt) as HP.
+    + admit.
+    + specialize (H HP).
+      destruct H as [H H']. destruct H as [H H''].
+      destruct HP as [HP HPP]. destruct HP as [HP HP'].
+      split.
+      * split.
+        ** auto.
+        ** apply H''. 
+      * split.
+        ** rewrite <- H. apply HPP. 
+        ** rewrite <- H. apply H'. *)
+  -  intros. exists s1. exists s2. 
+    admit.
+  Admitted.  
+
+Definition refinementUpdate (M1 : LayerImpl Op Op1) (M2 : LayerImpl Op Op1) (R1: relation LA1.(State) Lc.(State) unit) (R2: relation LA1.(State) Lc.(State) unit) :=
+  forall (T:Type) (p: proc Op1 T),
+  forall (c1 c2: Lc.(State)) (state : LA1.(State)) (r:T),
+  (exec Lc.(sem) (compile M1 p)) (c1) (c2) (r)  /\ R1 (state) (c1) (tt) -> exists (s1 s2 : Lc.(State)), exec Lc.(sem)  (compile M2 p) (s1) (s2) (r) /\ R2(state) (s1) (tt).  
+  
+
+Definition softwareUpdate(M1: LayerImpl Op  Op1) (M2: LayerImpl Op  COP):=
    forall (T: Type) (p1 p2 : proc Op1 T),
   exec Lc.(sem)  M1.(init) ;; exec Lc.(sem) (compile M1 p1) ;; shutdown ;;
   exec Lc.(sem)  (compile M2 (relinkingFunction p2))
@@ -62,7 +177,21 @@ Definition restrictiveSoftwareUpdate(M1: LayerImpl Op  Op1) (M2: LayerImpl Op  O
    exec Lc.(sem) M1.(init) ;; exec Lc.(sem) (compile M1 p1) ;; shutdown ;;
   exec Lc.(sem) (compile M1 p2).
 
+(** This will help us prove two base cases *)
+Theorem  CompileImpl : forall  (M1 : LayerImpl Op  Op1) (M2 : LayerImpl Op COP)
+  (T: Type) (p: proc Op1 T),
+  exec Lc.(sem) (compile M2 (relinkingFunction p))
+            --->
+            exec Lc.(sem) (compile M1 p).
+Proof.
+  Admitted.
+ 
 
-
+Theorem RSUProof :forall M1 M2: LayerImpl Op  Op1, restrictiveSoftwareUpdate M1 M2.
+Proof.
+  intros M1 M2. unfold restrictiveSoftwareUpdate. intros T p1 p2.
+  Admitted.   
+  
+  
 End Updates. 
 
