src/Examples/UpdateExamples/SmartContracts/compatibleUpdate.v
@@ -1,0 +1,35 @@
+Require Import Spec.update.
+Require Import Examples.UpdateExamples.SmartContracts.Firstversion.
+Require Import Examples.UpdateExamples.SmartContracts.version2.
+Require Import Spec.Proc.
+Require Import Spec.ProcTheorems.
+Require Import Helpers.RelationAlgebra.
+Require Import Helpers.RelationRewriting.
+Import  RelationNotations.
+
+
+About softwareUpdate.
+
+(**
+Record LayerImpl (C_Op Op0 : Type -> Type) : Type := Build_LayerImpl
+  { compile_op : forall T : Type, Op0 T -> proc C_Op T;
+    recover : proc C_Op unit;
+    init : proc C_Op InitStatus }.
+
+Arguments LayerImpl (C_Op Op)%function_scope
+Arguments Build_LayerImpl [C_Op]%function_scope (Op compile_op)%function_scope
+  recover init
+
+
+
+Print Firstversion.impl.
+
+Definition reldef: relation Firstversion.con.l.(Layer.State) Firstversion.con.l.(Layer.State) unit.
+Proof.
+  Admitted. 
+
+Lemma compatilbeSoftwareUpdate :
+  softwareUpdate (Firstversion.con.l) (reldef)  (Firstversion.impl) (version2.impl).
+Proof.                                                                                           Admitted. 
+
+ *)
