src/Examples/UpdateExamples/SmartContracts/version2.v
@@ -1,0 +1,491 @@
+From RecoveryRefinement Require Import Lib.
+Require Import Helpers.RelationRewriting.
+Require Import Spec.Hoare.
+Require Import Spec.HoareTactics.
+Require Import Spec.AbstractionSpec.
+Require Import Coq.Arith.Arith.
+Require Import Examples.UpdateExamples.SmartContracts.Firstversion. 
+Require Import Spec.update. 
+
+Module abs2. 
+
+  Definition State := nat%type.
+
+  Inductive O' : Type -> Type :=
+  | op_decrease (i : option nat) : O' unit.
+
+  About update.Op2. 
+
+  Definition Op2 := update.COP Firstversion.abs.Op O'.
+
+  Print Dynamics. (** (op: Type -> Type)  (State: Type) : Type *)
+
+  Definition DecCounter (i: nat) : State -> State :=
+    fun 'x => if  x-i <=? 0  then  0  else x-i.   
+ 
+
+  Definition test (T: Type) (op: Op2 T) :=
+    match op with
+    | O'case _ _ T o' =>  match o' with
+                      | op_decrease i => (match i with
+                             | Some i0 => True
+                             | None => True
+                                         end)
+                      end
+    | Op1case _  _ T op1   => match op1 with
+                             | abs.op_receive Msg => True
+                             | abs.op_observe => True
+                            end
+                                 
+    end. 
+  
+  Definition dynamics : Dynamics Op2 State :=
+    {| step T (op: Op2 T):=
+        match op with
+        | Op1case _ _ T op1 => match op1 with
+                        | abs.op_receive Msg => (match Msg with
+                             | Some (abs.Incr i) =>  puts (abs.IncrCounter i)
+                             | None => puts (abs.NoOp)
+                              end)
+                        | abs.op_observe  => reads (abs.read)
+                        end
+        | O'case _ _ T o' => match o' with
+                      | op_decrease i => (match i with
+                             | Some i0 => puts (DecCounter i0)
+                             | None => puts (abs.NoOp)
+                                         end)
+                      end
+       end;
+      crash_step := puts (fun 'x => 0); 
+    |}.
+
+  Definition l : Layer Op2 :=
+    {| Layer.State := State;
+       sem := dynamics;
+       initP := fun s => s = 0|}.
+End abs2. 
+
+(** OLD IMPL
+
+Definition impl : LayerImpl Firstversion.con.Op  abs.Op :=
+  {| compile_op T (op: abs.Op T) :=
+      match op with
+      | abs.op_receive Msg => match Msg with
+                             | Some (abs.Incr i) => update i
+                             | Some (abs.Decr i) =>
+                                 (currentVal <- read; 
+                                 _ <- (if currentVal - i <? 0 then noop
+                                 else write (currentVal - i)); Ret tt)%proc
+                               | None => noop
+                               end
+      | abs.op_observe => (val <- read; Ret (val)%nat)%proc
+       end;
+     recover := Ret tt;
+    init := Ret Initialized; |}.
+
+*)
+
+
+Definition impl : LayerImpl Firstversion.con.Op  abs2.Op2 :=
+  {| compile_op T (op: abs2.Op2 T) :=
+      match op with
+      | Op1case _ _ T op1 => Firstversion.impl.(compile_op) op1 
+      | O'case _ _ T o'  => match o' with
+                             | abs2.op_decrease i => (match i with
+                             | Some i0 => (currentVal <- read; 
+                                 _ <- (if currentVal - i0 <? 0 then noop
+                                 else write (currentVal - i0)); Ret tt)%proc
+                             | None => noop
+                                                end)
+                           end
+       end;
+     recover := Ret tt;
+    init := Ret Initialized; |}.
+
+Definition absr : relation abs2.l.(State) con.l.(State) unit :=
+  fun l s _ => l = s.
+
+
+(** --------------------- SPECS  ------------------------------------------*)
+
+Definition init_hspec : Specification InitStatus unit con.State :=
+  fun state =>
+    {|
+      pre := state = 0;
+      post := fun state' _ => state' = 0; 
+      alternate := fun state' (_:unit) => True;
+    |}.                            
+
+Definition receive_hspec (msg: option abs.Message) : Specification unit unit con.State :=
+  fun state =>
+    {|
+      pre := True;
+      post := fun state' (_:unit) => match msg with
+                              | Some (abs.Incr i) => state' = state + i
+                              | None => state' = state
+                              end;
+      alternate := fun state' (_:unit) => state' = 0;
+    |}.
+
+Definition receive_rspec (msg: option abs.Message) : Specification unit unit con.State :=
+  fun state =>
+    {|
+      pre := True;
+      post := fun state' (_:unit) => match msg with
+                              | Some (abs.Incr i) => state' = state + i
+                              | None => state' = state
+                              end;
+      alternate := fun state' (_:unit) => state' = 0;
+    |}.
+
+Definition observe_hspec : Specification nat unit con.State :=
+  fun state =>
+    {|
+      pre := True;
+      post := fun state' v => state' = state /\ v = state;
+      alternate := fun state' v => state' = 0;
+    |}.
+
+Definition observe_rspec : Specification nat unit con.State :=
+  fun state =>
+    {|
+      pre := True;
+      post := fun state' v => state' = state /\ v = state;
+      alternate := fun state' v => state' = 0;
+    |}.
+
+Definition recover_spec : Specification unit unit con.State :=
+  fun state =>
+    {|
+      pre := state = 0;
+      post := fun state' (_:unit) => state' = 0;
+      alternate := fun state' (_:unit) => state' = 0;
+    |}.
+
+Definition decrease_rspec (i: option nat) :  Specification unit unit con.State :=
+  fun state =>
+    {|
+      pre := True;
+      post :=  fun state' (_:unit) => match i with
+                               | Some i0 => (state - i0 < 0 -> state' = state) /\ (state - i0 >= 0 -> state' = state - i0)
+                               | None => state' = state
+                               end;
+      alternate :=fun state' (_:unit) => state' = 0;
+      |}. 
+
+Definition decrease_hspec (i: option nat) :  Specification unit unit con.State :=
+  fun state =>
+    {|
+      pre := True;
+      post :=  fun state' (_:unit) => match i with
+                               | Some i0 => (state - i0 < 0 -> state' = state) /\ (state - i0 >= 0 -> state' = state - i0)
+                               | None => state' = state
+                               end;
+      alternate :=fun state' (_:unit) => state' = 0;
+      |}.
+
+
+(** --------------------- TACTICS  ------------------------------------------*)
+
+Ltac simplify :=
+  repeat match goal with
+         | |- forall _, _ => intros
+         | _ => deex
+         | _ => destruct_tuple
+         | _ => destruct_tuple
+         | [ H: reads _ _ _ _ |- _] => unfold reads in H
+         | [ H: puts _ _ _ _ |- _] => unfold puts in H
+         | [ u: unit |- _ ] => destruct u
+         | |- _ /\ _ => split; [ solve [auto] | ]
+         | |- _ /\ _ => split; [ | solve [auto] ]
+         | _ => progress simpl in *
+         | _ => progress safe_intuition
+         | _ => progress subst
+         | _ => progress autorewrite with array in *
+end.
+
+Ltac extract_post :=
+  lazymatch goal with
+  | |- pre _ => simpl
+  | |- alternate _ _ _ => simpl
+  | |- post _ _ _ => simpl
+  | _ => idtac
+  end.
+
+Lemma op_step_crash T (op: con.Op T) u s' r :
+  (op_spec con.dynamics op u).(alternate) s' r ->
+  s' = 0.
+Proof.
+  intros.
+  hnf in H; propositional.
+  destruct H0; propositional.
+Qed.
+
+Lemma crash_step_simp s s' r :
+  con.dynamics.(crash_step) s s' r ->
+  s' = 0.
+Proof.
+  compute; auto.
+Qed.
+
+Ltac extract_crash H :=
+  lazymatch type of H with
+  | con.dynamics.(crash_step) _ _ _ =>
+    apply crash_step_simp in H; subst
+  | (op_spec con.dynamics _ _).(alternate) _ _ =>
+    apply op_step_crash in H; subst
+  | _ => idtac
+  end.
+
+Ltac extract_pre H :=
+  let P := type of H in
+  match eval hnf in P with
+  | True => clear H
+  | ?v = _ =>
+    is_var v;
+    hnf in H; subst
+  | (?v = _) /\ _ =>
+    is_var v;
+    hnf in H;
+    let Heq := fresh "Heq" in
+    destruct H as (Heq&H); subst
+  | _ => idtac
+  end.
+
+Ltac step_ret :=
+  apply ret_hspec; cbn [pre post alternate];
+  (let H := fresh "Hpre" in
+   intros * H; extract_pre H);
+  apply conj;
+  [ extract_post
+  | let H := fresh "Hcrash" in
+    intros * H; extract_crash H; extract_post ].
+
+Lemma util_and3 (P Q R:Prop) :
+  P -> Q -> R -> P /\ Q /\ R.
+Proof. firstorder. Qed.
+
+Ltac step_bind :=
+  eapply proc_hspec_rx; [ solve [ eauto ] | cbn [pre post alternate] .. ];
+  (let H := fresh "Hpre" in
+   intros * H; extract_pre H);
+  apply util_and3;
+  swap 1 2;
+  [ intros
+  | extract_post
+  | let H := fresh "Hcrash" in
+    intros * H; extract_crash H;
+    extract_post ].
+
+Ltac newstep :=
+  monad_simpl;
+  lazymatch goal with
+  | |- proc_hspec _ (compile_op _ _) _ => simpl
+  | |- proc_hspec _ (Ret _) _ => step_ret
+  | |- proc_hspec _ (Bind _ _) _ => step_bind
+  end.
+
+(** --------------------- PROOFS ------------------------------------------*)
+
+Lemma recover_cok : proc_hspec con.dynamics (impl.(recover)) recover_spec.
+Proof. simpl. eapply ret_hspec; firstorder. Qed.
+
+Lemma recover_idempotent :
+  idempotent (fun (t: unit) => recover_spec).
+Proof.
+  unfold idempotent; intuition; exists tt; simpl in *.
+  unfold puts in *; firstorder; congruence.
+Qed.
+
+Global Hint Resolve recover_cok recover_idempotent : core.
+
+Lemma recover_rok : proc_rspec con.dynamics (impl.(recover)) (impl.(recover)) recover_spec.
+Proof. eapply proc_hspec_to_rspec; eauto. intros []; eauto. Qed.
+
+Lemma init_cok:
+  proc_hspec con.dynamics (impl.(init)) (init_hspec).
+Proof.
+  eapply ret_hspec; firstorder. Qed.
+
+
+(**Lemma decrease_cok : proc_hspec con.dynamics (impl.(compile_op) (abs2.Op2 (abs2.op_decrease) )) (decrease_hspec).
+Proof.
+Admitted.
+
+Lemma decrease_ok : proc_rspec con.dynamics (impl.(compile_op) (abs2.op_decrease)) impl.(recover) (decrease_rspec).
+Proof.
+Admitted. *)
+
+Lemma decrease1_ok : forall (n:nat) (sC: con.State),   proc_rspec con.dynamics
+    (currentVal <- read; _ <- write (currentVal - n); Ret tt)%proc 
+    (Ret tt) (decrease_rspec (Some n)).
+Proof.
+  intros. unfold proc_rspec. unfold rimpl. simpl. split.
+  * intros. unfold spec_exec. unfold decrease_rspec. simpl. intros.
+    unfold and_then in H. destruct H as [o1 H]. destruct H as [y0 H]. destruct H as [H1 H2]. destruct H2 as [o2 H2]. destruct H2 as [y1 H2]. unfold reads in H1. unfold con.get in H1. destruct H1 as [H1 H3].
+    unfold puts in H2. unfold con.set in H2. unfold pure in H2. destruct H2 as [H2 H4]. destruct H4 as [H4 H5].  split.
+    ** intros. rewrite -> H1 in H2. admit. 
+    ** intros.  rewrite -> H1 in H2. rewrite -> H4 in H2. auto. 
+  * intros. unfold spec_aexec. unfold decrease_rspec. simpl. intros. unfold rexec in H. unfold and_then in H. destruct H as [o1 [y0 H]]. induction H. unfold exec_recover in H1. unfold and_then in H1. destruct H1 as [o1' [y1' [H1 H3]]].  unfold exec in H3. unfold pure in H3. induction H1.
+    ** unfold exec_crash in H. unfold rel_or in H. simpl in H. unfold puts in H. unfold and_then in H. destruct H.
+       *** destruct H.
+           **** destruct H3 as [H3 H4]. rewrite -> H in H3. inversion H3. reflexivity.
+          **** destruct H as [o2 [y1 H]]. unfold reads in H. destruct H as [H1 H]. destruct H3 as [H3 H4]. rewrite -> H in H3. inversion H3. reflexivity.
+       *** destruct H as [o2 [y1 H]]. unfold reads in H. unfold con.get in H. destruct H as [H6 H]. destruct H.
+           **** destruct H. {destruct H3 as [H3 H4]. rewrite -> H in H3. inversion H3. reflexivity.} {destruct H. destruct H. destruct H as [H5 H]. destruct H3 as [H3 H4]. rewrite -> H in H3. inversion H3. reflexivity.}
+           ****  destruct H. destruct H. destruct H as [H5 H]. destruct H3 as [H3 H4]. rewrite -> H in H3. inversion H3. reflexivity.
+   ** 
+Admitted.
+
+Lemma decrease2_ok : forall sC: con.State, proc_rspec con.dynamics noop (Ret tt) (decrease_rspec None).
+Proof.
+Admitted.
+
+
+Global Hint Resolve init_cok receive_ok observe_ok : core. 
+ 
+
+Definition rf : LayerRefinement con.l abs2.l.
+Proof.
+  refine {| Layer.impl := impl;
+           Layer.absr := absr; |}.
+  - (** compile op refines step *)
+    red; intros. destruct op.
+    +  destruct o.
+      ++ (** op = receive *)
+      eapply proc_rspec_crash_refines_op  with (spec := receive_rspec Msg); eauto; unfold spec_impl, absr in *; simplify.
+      * eapply proc_rspec_impl with (spec1 := receive_rspec Msg).
+        ** unfold spec_impl. simplify. split.
+           *** intros. exists s'. split.
+               { auto. }
+               { destruct Msg.
+                 {destruct m.
+                  **** auto.}
+                 { auto. }}
+           *** intros. exists s'. split. { auto. }  { auto. }
+        ** eapply receive_ok. 
+      * destruct Msg.
+        ** destruct m.
+           *** unfold puts. unfold abs.IncrCounter. auto.
+        ** unfold abs.NoOp. unfold puts. auto. 
+    ++ (** op = observe *)
+      eapply proc_rspec_crash_refines_op  with (spec := observe_rspec); eauto; unfold spec_impl, absr in *; simplify.
+      * eapply proc_rspec_impl with (spec1 :=  observe_rspec).
+        ** unfold spec_impl. simplify. split.
+           *** intros. exists s'. destruct H as [H H']. split.
+               **** auto. 
+               **** split. { auto. } { auto. } 
+           *** intros. exists s'. split.
+               **** auto.
+               **** auto. 
+        ** eapply observe_ok.  
+      * unfold reads.  unfold abs.read. split.  { auto. } { auto. }
+    + destruct o. eapply proc_rspec_crash_refines_op  with (spec := decrease_rspec i); eauto; unfold spec_impl, absr in *; simplify.
+      * eapply proc_rspec_impl with (spec1 := decrease_rspec i).
+        ** unfold spec_impl. simplify. split.
+           *** intros. exists s'. split.
+               { auto. }
+               { destruct i.  { apply H. } {auto. }
+                 }
+           *** intros.  exists s'. split. { auto. }  { auto. }
+        ** destruct i.
+           *** apply decrease1_ok. auto. 
+           *** apply decrease2_ok.  auto.  
+      * destruct i.
+        ** unfold puts. unfold abs2.DecCounter. destruct (sA - n).
+           *** simpl. destruct H0 as [H0 H1]. assert (0 >= 0) as H2.
+               { auto.} { specialize (H1 H2). auto. }
+           *** simpl. destruct H0 as [H0 H1]. assert (S n0 >= 0) as H.
+               { auto. apply le_0_n. } { specialize (H1 H). auto. } 
+        ** unfold puts. unfold abs.NoOp. auto.  
+  - (** recovery refines crash step *)
+    eapply proc_rspec_recovery_refines_crash_step; [ intros; eapply recover_rok |..]; simplify. Print tt. 
+    intuition; exists 0; unfold absr in *; simplify; intuition; subst; simplify; try congruence. 
+  - (** init step *)
+    eapply proc_hspec_init_ok with (spec := init_hspec).
+    * unfold impl. simpl. eapply init_cok. 
+    * intros. unfold init_hspec. simpl. unfold con.l in H. simpl in H. auto. 
+    * intros. exists 0. unfold absr. unfold abs.l. simpl.
+      unfold init_hspec in H.  simpl in H. split.
+      ** auto.
+      ** auto.
+Qed. 
+
+
+
+
+(**
+ Inductive Op : Type -> Type :=
+  | op1case (T:Type) : Op1 T -> Op T
+  | o'case  (T:Type) : O' T -> Op T.
+
+ Inductive  Op2: Type -> Type :=
+  | Op1case(T:Type) : Op1 T -> Op2 T
+  | O'case(T:Type) : O' T -> Op2 T.
+
+  Inductive Op1 : Type -> Type :=
+  | op_receive (Msg : option Message) : Op1 unit
+  | op_observe : Op1 nat. 
+
+Inductive  Op2: Type -> Type :=
+| Op1case(T:Type) : Op1 T -> Op2 T
+| O'case(T:Type) : O' T -> Op2 T.
+
+  Inductive OpTest : Type -> Type :=
+  | op1case2 (T : Type) (op : Op1 T) : OpTest T
+  | o'case2 (T : Type) (op : O' T) : OpTest T.
+
+  Definition  opTest_step (T:Type) (op: OpTest T) : OpSemantics OpTest State :=
+    match op with
+    | op1case2 op1 => (match op1 with
+        | op_receive Msg => (match Msg with
+                             | Some (Incr i) =>  puts (IncrCounter i)
+                             | None => puts (NoOp)
+                              end)
+        | op_observe  => reads (read)
+                      end)
+    | o'case2 o' => (match o' with
+        | op_decrease i => (match i with
+                       | Some i0 => puts (DecCounter i0)
+                       | None => NoOp
+                           end)
+                    end)
+    end.
+
+   *)
+
+  (** Inductive o'_step : OpSemantics O' State :=
+  | step_decrease : forall i: option nat, forall state state',
+    match i with
+    | Some i0 => state' = ((DecCounter i0) state)
+    | None => state' = state
+    end ->
+    o'_step (op_decrease i) state state' tt. *)
+
+  (** ATTEMPT 1 : DIDN'T WORK 
+
+ Definition relinkO'{T:Type} (o' : O' T) : Op T :=
+    match o' with
+    | op_decrease i => (match i with
+                       | Some i0 => puts (DecCounter i0)
+                       | None => NoOp
+                       end)
+    end. 
+
+  Definition relinkOp1{T:Type} (op1: Firstversion.abs.Op T) : Op T :=
+    match op1 with
+    | op_receive Msg => (match Msg with
+                             | Some (Incr i) =>  puts (IncrCounter i)
+                             | None => puts (NoOp)
+                              end)
+    | op_observe  => reads (read)
+    end.
+
+ *)
+(**  Inductive op_step : OpSemantics Op State :=
+ | step_op1 :forall (T:Type) (op: Op1 T) (state state' : State) (res: T),
+    Firstversion.abs.op1_step op state state' res ->
+    op_step (op1case op) state state' res
+  | step_o' :  forall (T: Type) (op: O' T) (state state': State) (res: T),
+      o'_step op state state' res ->
+      op_step (o'case op) state state' res. *)
